Clean/Examples/FemtoCairo/FlatAirRust.lean
@@ -7,9 +7,6 @@ open Examples.FemtoCairo
 open Examples.FemtoCairo.Types
 open Examples.FemtoCairo.Plonky3MemoryTestData
 
-private def memoryValues : Fin 8 → F pBabybear := fun i =>
-  (#v[0, 5, 3, 7, 2, 10, 0, 0] : Vector (F pBabybear) 8)[i]
-
 private theorem h_memorySize : 8 < pBabybear := by native_decide
 
 def main : IO Unit := do
@@ -17,6 +14,7 @@ def main : IO Unit := do
       "FemtoCairoFlatAirProgram"
       (Examples.FemtoCairo.FlatAir.soundEnsemble testProgram h_programSize h_memorySize
         initialState).ensemble
-      (Examples.FemtoCairo.FlatAir.Witness.config testProgram memoryValues initialState 8 1000) with
+      (Examples.FemtoCairo.FlatAir.Witness.config (memorySize := 8)
+        testProgram initialState 8 1000) with
   | .ok rust => IO.print rust
   | .error error => throw (IO.userError error)
